A12Kernel.lean
@@ -146,6 +146,7 @@ import A12Kernel.Elaboration.StringComputationRun
 import A12Kernel.Elaboration.StringComputationRunRelation
 import A12Kernel.Elaboration.StringComputationRunResult
 import A12Kernel.Elaboration.StringComputationRunApplication
+import A12Kernel.Elaboration.AddressedFieldValueAsString
 import A12Kernel.Elaboration.NumberToStringComputationRun
 import A12Kernel.Elaboration.StringToNumberComputationRun
 import A12Kernel.Elaboration.ScalarComputationRun
